doc/tools.hs
@@ -1,0 +1,9 @@
+display :: Prelude.String -> SState a b c -> SState a b c
+display label k ss@(Build_SSInfo sd _) =
+    case IState.runIState k
+             (trace (label GHC.Base.++ " - sd: "
+                           GHC.Base.++ Prelude.show sd) ss) of
+        Prelude.Left e -> Prelude.error (Prelude.show e)
+        x@(Prelude.Right (_, Build_SSInfo sd' _)) ->
+            trace (label GHC.Base.++ " - sd': "
+                         GHC.Base.++ Prelude.show sd') x
