test/Main.hs
@@ -16,222 +16,222 @@ import Test.Hspec
 
 main :: IO ()
 main = hspec $ do
-    let basicAlloc = regs $ alloc 2 0 >> alloc 1 1 >> alloc 0 2
+  let basicAlloc = regs $ alloc 2 0 >> alloc 1 1 >> alloc 0 2
 
-    describe "Sanity tests" $ do
-        it "Single instruction" $ asmTest
-            (add v0 v1 v2)
+  describe "Sanity tests" $ do
+    it "Single instruction" $ asmTest
+        (add v0 v1 v2)
 
-            basicAlloc
+        basicAlloc
 
-        it "Single, repeated instruction" $ asmTest
-            (do add v0 v1 v2
-                add v0 v1 v2
-                add v0 v1 v2) $ do
+    it "Single, repeated instruction" $ asmTest
+        (do add v0 v1 v2
+            add v0 v1 v2
+            add v0 v1 v2) $ do
 
-            basicAlloc
-            basicAlloc
-            basicAlloc
+        basicAlloc
+        basicAlloc
+        basicAlloc
 
-        it "Multiple instructions" $ asmTest
-            (do add v0 v1 v2
-                add v0 v1 v3
-                add v0 v1 v2) $ do
+    it "Multiple instructions" $ asmTest
+        (do add v0 v1 v2
+            add v0 v1 v3
+            add v0 v1 v2) $ do
 
-            basicAlloc
-            regs $ alloc 3 3 >> alloc 1 1 >> alloc 0 2
-            basicAlloc
+        basicAlloc
+        regs $ alloc 3 3 >> alloc 1 1 >> alloc 0 2
+        basicAlloc
 
-        it "More variables used than registers" $ asmTest
-            (do add v0 v1 v2
-                add v3 v4 v5
-                add v6 v7 v8
-                add v9 v10 v11
-                add v12 v13 v14
-                add v15 v16 v17
-                add v18 v19 v20
-                add v21 v22 v23
-                add v24 v25 v26
-                add v27 v28 v29
-                add v30 v31 v32
-                add v33 v34 v35) $ do
+    it "More variables used than registers" $ asmTest
+        (do add v0 v1 v2
+            add v3 v4 v5
+            add v6 v7 v8
+            add v9 v10 v11
+            add v12 v13 v14
+            add v15 v16 v17
+            add v18 v19 v20
+            add v21 v22 v23
+            add v24 v25 v26
+            add v27 v28 v29
+            add v30 v31 v32
+            add v33 v34 v35) $ do
 
-            regs $ alloc  2 0 >> alloc  1 1 >> alloc  0 2
-            regs $ alloc  5 0 >> alloc  4 1 >> alloc  3 2
-            regs $ alloc  8 0 >> alloc  7 1 >> alloc  6 2
-            regs $ alloc 11 0 >> alloc 10 1 >> alloc  9 2
-            regs $ alloc 14 0 >> alloc 13 1 >> alloc 12 2
-            regs $ alloc 17 0 >> alloc 16 1 >> alloc 15 2
-            regs $ alloc 20 0 >> alloc 19 1 >> alloc 18 2
-            regs $ alloc 23 0 >> alloc 22 1 >> alloc 21 2
-            regs $ alloc 26 0 >> alloc 25 1 >> alloc 24 2
-            regs $ alloc 29 0 >> alloc 28 1 >> alloc 27 2
-            regs $ alloc 32 0 >> alloc 31 1 >> alloc 30 2
-            regs $ alloc 35 0 >> alloc 34 1 >> alloc 33 2
+        regs $ alloc  2 0 >> alloc  1 1 >> alloc  0 2
+        regs $ alloc  5 0 >> alloc  4 1 >> alloc  3 2
+        regs $ alloc  8 0 >> alloc  7 1 >> alloc  6 2
+        regs $ alloc 11 0 >> alloc 10 1 >> alloc  9 2
+        regs $ alloc 14 0 >> alloc 13 1 >> alloc 12 2
+        regs $ alloc 17 0 >> alloc 16 1 >> alloc 15 2
+        regs $ alloc 20 0 >> alloc 19 1 >> alloc 18 2
+        regs $ alloc 23 0 >> alloc 22 1 >> alloc 21 2
+        regs $ alloc 26 0 >> alloc 25 1 >> alloc 24 2
+        regs $ alloc 29 0 >> alloc 28 1 >> alloc 27 2
+        regs $ alloc 32 0 >> alloc 31 1 >> alloc 30 2
+        regs $ alloc 35 0 >> alloc 34 1 >> alloc 33 2
 
-        it "Single long-lived variable" $ asmTest
-            (do add v0 v1 v2
-                add v0 v4 v5
-                add v0 v7 v8
-                add v0 v10 v11) $ do
+    it "Single long-lived variable" $ asmTest
+        (do add v0 v1 v2
+            add v0 v4 v5
+            add v0 v7 v8
+            add v0 v10 v11) $ do
 
-            regs $ alloc  2 0 >> alloc  1 1 >> alloc  0 2
-            regs $ alloc  5 0 >> alloc  4 1 >> alloc  0 2
-            regs $ alloc  8 0 >> alloc  7 1 >> alloc  0 2
-            regs $ alloc 11 0 >> alloc 10 1 >> alloc  0 2
+        regs $ alloc  2 0 >> alloc  1 1 >> alloc  0 2
+        regs $ alloc  5 0 >> alloc  4 1 >> alloc  0 2
+        regs $ alloc  8 0 >> alloc  7 1 >> alloc  0 2
+        regs $ alloc 11 0 >> alloc 10 1 >> alloc  0 2
 
-        it "Two long-lived variables" $ asmTest
-            (do add v0 v1 v2
-                add v0 v4 v5
-                add v0 v4 v8
-                add v0 v4 v11) $ do
+    it "Two long-lived variables" $ asmTest
+        (do add v0 v1 v2
+            add v0 v4 v5
+            add v0 v4 v8
+            add v0 v4 v11) $ do
 
-            regs $ alloc  2 0 >> alloc  1 1 >> alloc  0 2
-            regs $ alloc  5 0 >> alloc  4 1 >> alloc  0 2
-            regs $ alloc  8 0 >> alloc  4 1 >> alloc  0 2
-            regs $ alloc 11 0 >> alloc  4 1 >> alloc  0 2
+        regs $ alloc  2 0 >> alloc  1 1 >> alloc  0 2
+        regs $ alloc  5 0 >> alloc  4 1 >> alloc  0 2
+        regs $ alloc  8 0 >> alloc  4 1 >> alloc  0 2
+        regs $ alloc 11 0 >> alloc  4 1 >> alloc  0 2
 
-        it "More variables used than registers" $ asmTest
-            (do add v0 v1 v2
-                add v3 v4 v5
-                add v6 v7 v8
-                add v9 v10 v11
-                add v12 v13 v14
-                add v15 v16 v17
-                add v18 v19 v20
-                add v21 v22 v23
-                add v24 v25 v26
-                add v27 v28 v29
-                add v30 v31 v32
-                add v33 v34 v35) $ do
+    it "More variables used than registers" $ asmTest
+        (do add v0 v1 v2
+            add v3 v4 v5
+            add v6 v7 v8
+            add v9 v10 v11
+            add v12 v13 v14
+            add v15 v16 v17
+            add v18 v19 v20
+            add v21 v22 v23
+            add v24 v25 v26
+            add v27 v28 v29
+            add v30 v31 v32
+            add v33 v34 v35) $ do
 
-            regs $ alloc  2 0 >> alloc  1 1 >> alloc  0 2
-            regs $ alloc  5 0 >> alloc  4 1 >> alloc  3 2
-            regs $ alloc  8 0 >> alloc  7 1 >> alloc  6 2
-            regs $ alloc 11 0 >> alloc 10 1 >> alloc  9 2
-            regs $ alloc 14 0 >> alloc 13 1 >> alloc 12 2
-            regs $ alloc 17 0 >> alloc 16 1 >> alloc 15 2
-            regs $ alloc 20 0 >> alloc 19 1 >> alloc 18 2
-            regs $ alloc 23 0 >> alloc 22 1 >> alloc 21 2
-            regs $ alloc 26 0 >> alloc 25 1 >> alloc 24 2
-            regs $ alloc 29 0 >> alloc 28 1 >> alloc 27 2
-            regs $ alloc 32 0 >> alloc 31 1 >> alloc 30 2
-            regs $ alloc 35 0 >> alloc 34 1 >> alloc 33 2
+        regs $ alloc  2 0 >> alloc  1 1 >> alloc  0 2
+        regs $ alloc  5 0 >> alloc  4 1 >> alloc  3 2
+        regs $ alloc  8 0 >> alloc  7 1 >> alloc  6 2
+        regs $ alloc 11 0 >> alloc 10 1 >> alloc  9 2
+        regs $ alloc 14 0 >> alloc 13 1 >> alloc 12 2
+        regs $ alloc 17 0 >> alloc 16 1 >> alloc 15 2
+        regs $ alloc 20 0 >> alloc 19 1 >> alloc 18 2
+        regs $ alloc 23 0 >> alloc 22 1 >> alloc 21 2
+        regs $ alloc 26 0 >> alloc 25 1 >> alloc 24 2
+        regs $ alloc 29 0 >> alloc 28 1 >> alloc 27 2
+        regs $ alloc 32 0 >> alloc 31 1 >> alloc 30 2
+        regs $ alloc 35 0 >> alloc 34 1 >> alloc 33 2
 
-        it "One variable with a long interval" $ asmTest
-            (do add v0   v1  v2
-                add v3   v4  v5
-                add v6   v7  v8
-                add v9  v10 v11
-                add v12 v13 v14
-                add v15 v16 v17
-                add v18 v19 v20
-                add v21 v22 v23
-                add v24 v25 v26
-                add v27 v28 v29
-                add v30 v31 v32
-                add v0  v34 v35) $ do
+    it "One variable with a long interval" $ asmTest
+        (do add v0   v1  v2
+            add v3   v4  v5
+            add v6   v7  v8
+            add v9  v10 v11
+            add v12 v13 v14
+            add v15 v16 v17
+            add v18 v19 v20
+            add v21 v22 v23
+            add v24 v25 v26
+            add v27 v28 v29
+            add v30 v31 v32
+            add v0  v34 v35) $ do
 
-            regs $ alloc  2 0 >> alloc  1 1 >> alloc  0 2
-            regs $ alloc  5 0 >> alloc  4 1 >> alloc  3 3
-            regs $ alloc  8 0 >> alloc  7 1 >> alloc  6 3
-            regs $ alloc 11 0 >> alloc 10 1 >> alloc  9 3
-            regs $ alloc 14 0 >> alloc 13 1 >> alloc 12 3
-            regs $ alloc 17 0 >> alloc 16 1 >> alloc 15 3
-            regs $ alloc 20 0 >> alloc 19 1 >> alloc 18 3
-            regs $ alloc 23 0 >> alloc 22 1 >> alloc 21 3
-            regs $ alloc 26 0 >> alloc 25 1 >> alloc 24 3
-            regs $ alloc 29 0 >> alloc 28 1 >> alloc 27 3
-            regs $ alloc 32 0 >> alloc 31 1 >> alloc 30 3
-            regs $ alloc 35 0 >> alloc 34 1 >> alloc  0 2
+        regs $ alloc  2 0 >> alloc  1 1 >> alloc  0 2
+        regs $ alloc  5 0 >> alloc  4 1 >> alloc  3 3
+        regs $ alloc  8 0 >> alloc  7 1 >> alloc  6 3
+        regs $ alloc 11 0 >> alloc 10 1 >> alloc  9 3
+        regs $ alloc 14 0 >> alloc 13 1 >> alloc 12 3
+        regs $ alloc 17 0 >> alloc 16 1 >> alloc 15 3
+        regs $ alloc 20 0 >> alloc 19 1 >> alloc 18 3
+        regs $ alloc 23 0 >> alloc 22 1 >> alloc 21 3
+        regs $ alloc 26 0 >> alloc 25 1 >> alloc 24 3
+        regs $ alloc 29 0 >> alloc 28 1 >> alloc 27 3
+        regs $ alloc 32 0 >> alloc 31 1 >> alloc 30 3
+        regs $ alloc 35 0 >> alloc 34 1 >> alloc  0 2
 
-        it "Many variables with long intervals" $ asmTest
-            (do add v0   v1  v2
-                add v3   v4  v5
-                add v6   v7  v8
-                add v9  v10 v11
-                add v12 v13 v14
-                add v15 v16 v17
-                add v18 v19 v20
-                add v21 v22 v23
-                add v24 v25 v26
-                add v27 v28 v29
-                add v0   v1  v2
-                add v3   v4  v5
-                add v6   v7  v8
-                add v9  v10 v11
-                add v12 v13 v14
-                add v15 v16 v17
-                add v18 v19 v20
-                add v21 v22 v23
-                add v24 v25 v26
-                add v27 v28 v29
-            ) $ do
+    it "Many variables with long intervals" $ asmTest
+        (do add v0   v1  v2
+            add v3   v4  v5
+            add v6   v7  v8
+            add v9  v10 v11
+            add v12 v13 v14
+            add v15 v16 v17
+            add v18 v19 v20
+            add v21 v22 v23
+            add v24 v25 v26
+            add v27 v28 v29
+            add v0   v1  v2
+            add v3   v4  v5
+            add v6   v7  v8
+            add v9  v10 v11
+            add v12 v13 v14
+            add v15 v16 v17
+            add v18 v19 v20
+            add v21 v22 v23
+            add v24 v25 v26
+            add v27 v28 v29
+        ) $ do
 
-            regs $ alloc  2  0 >> alloc  1  1 >> alloc  0  2
-            regs $ alloc  5  3 >> alloc  4  4 >> alloc  3  5
-            regs $ alloc  8  6 >> alloc  7  7 >> alloc  6  8
-            regs $ alloc 11  9 >> alloc 10 10 >> alloc  9 11
-            regs $ alloc 14 12 >> alloc 13 13 >> alloc 12 14
-            regs $ alloc 17 15 >> alloc 16 16 >> alloc 15 17
-            regs $ alloc 20 18 >> alloc 19 19 >> alloc 18 20
-            regs $ alloc 23 21 >> alloc 22 22 >> alloc 21 23
-            regs $ alloc 26 24 >> alloc 25 25 >> alloc 24 26
-            regs $ alloc 29 27 >> alloc 28 28 >> alloc 27 29
-            regs $ alloc  2  0 >> alloc  1  1 >> alloc  0  2
-            regs $ alloc  5  3 >> alloc  4  4 >> alloc  3  5
-            regs $ alloc  8  6 >> alloc  7  7 >> alloc  6  8
-            regs $ alloc 11  9 >> alloc 10 10 >> alloc  9 11
-            regs $ alloc 14 12 >> alloc 13 13 >> alloc 12 14
-            regs $ alloc 17 15 >> alloc 16 16 >> alloc 15 17
-            regs $ alloc 20 18 >> alloc 19 19 >> alloc 18 20
-            regs $ alloc 23 21 >> alloc 22 22 >> alloc 21 23
-            regs $ alloc 26 24 >> alloc 25 25 >> alloc 24 26
-            regs $ alloc 29 27 >> alloc 28 28 >> alloc 27 29
+        regs $ alloc  2  0 >> alloc  1  1 >> alloc  0  2
+        regs $ alloc  5  3 >> alloc  4  4 >> alloc  3  5
+        regs $ alloc  8  6 >> alloc  7  7 >> alloc  6  8
+        regs $ alloc 11  9 >> alloc 10 10 >> alloc  9 11
+        regs $ alloc 14 12 >> alloc 13 13 >> alloc 12 14
+        regs $ alloc 17 15 >> alloc 16 16 >> alloc 15 17
+        regs $ alloc 20 18 >> alloc 19 19 >> alloc 18 20
+        regs $ alloc 23 21 >> alloc 22 22 >> alloc 21 23
+        regs $ alloc 26 24 >> alloc 25 25 >> alloc 24 26
+        regs $ alloc 29 27 >> alloc 28 28 >> alloc 27 29
+        regs $ alloc  2  0 >> alloc  1  1 >> alloc  0  2
+        regs $ alloc  5  3 >> alloc  4  4 >> alloc  3  5
+        regs $ alloc  8  6 >> alloc  7  7 >> alloc  6  8
+        regs $ alloc 11  9 >> alloc 10 10 >> alloc  9 11
+        regs $ alloc 14 12 >> alloc 13 13 >> alloc 12 14
+        regs $ alloc 17 15 >> alloc 16 16 >> alloc 15 17
+        regs $ alloc 20 18 >> alloc 19 19 >> alloc 18 20
+        regs $ alloc 23 21 >> alloc 22 22 >> alloc 21 23
+        regs $ alloc 26 24 >> alloc 25 25 >> alloc 24 26
+        regs $ alloc 29 27 >> alloc 28 28 >> alloc 27 29
 
-        it "Induce spillage of one variable" $ asmTest
-            (do add v0   v1  v2
-                add v3   v4  v5
-                add v6   v7  v8
-                add v9  v10 v11
-                add v12 v13 v14
-                add v15 v16 v17
-                add v18 v19 v20
-                add v21 v22 v23
-                add v24 v25 v26
-                add v27 v28 v29
-                add v30 v31 v32
-                add v0   v1  v2
-                add v3   v4  v5
-                add v6   v7  v8
-                add v9  v10 v11
-                add v12 v13 v14
-                add v15 v16 v17
-                add v18 v19 v20
-                add v21 v22 v23
-                add v24 v25 v26
-                add v27 v28 v29
-                add v30 v31 v32) $ do
+    it "Induce spillage of one variable" $ asmTest
+        (do {-  1 -} add v0   v1  v2
+            {-  3 -} add v3   v4  v5
+            {-  5 -} add v6   v7  v8
+            {-  7 -} add v9  v10 v11
+            {-  9 -} add v12 v13 v14
+            {- 11 -} add v15 v16 v17
+            {- 13 -} add v18 v19 v20
+            {- 15 -} add v21 v22 v23
+            {- 17 -} add v24 v25 v26
+            {- 19 -} add v27 v28 v29
+            {- 21 -} add v30 v31 v32
+            {- 23 -} add v0   v1  v2
+            {- 25 -} add v3   v4  v5
+            {- 27 -} add v6   v7  v8
+            {- 29 -} add v9  v10 v11
+            {- 31 -} add v12 v13 v14
+            {- 33 -} add v15 v16 v17
+            {- 35 -} add v18 v19 v20
+            {- 37 -} add v21 v22 v23
+            {- 39 -} add v24 v25 v26
+            {- 41 -} add v27 v28 v29
+            {- 43 -} add v30 v31 v32) $ do
 
-            regs $ alloc  2  0 >> alloc  1  1 >> alloc  0  2
-            regs $ alloc  5  3 >> alloc  4  4 >> alloc  3  5
-            regs $ alloc  8  6 >> alloc  7  7 >> alloc  6  8
-            regs $ alloc 11  9 >> alloc 10 10 >> alloc  9 11
-            regs $ alloc 14 12 >> alloc 13 13 >> alloc 12 14
-            regs $ alloc 17 15 >> alloc 16 16 >> alloc 15 17
-            regs $ alloc 20 18 >> alloc 19 19 >> alloc 18 20
-            regs $ alloc 23 21 >> alloc 22 22 >> alloc 21 23
-            regs $ alloc 26 24 >> alloc 25 25 >> alloc 24 26
-            regs $ alloc 29 27 >> alloc 28 28 >> alloc 27 29
-            regs $ alloc 32 30 >> alloc 31 31 >> alloc 30 32
-            regs $ alloc  2  0 >> alloc  1  1 >> alloc  0  2
-            regs $ alloc  5  3 >> alloc  4  4 >> alloc  3  5
-            regs $ alloc  8  6 >> alloc  7  7 >> alloc  6  8
-            regs $ alloc 11  9 >> alloc 10 10 >> alloc  9 11
-            regs $ alloc 14 12 >> alloc 13 13 >> alloc 12 14
-            regs $ alloc 17 15 >> alloc 16 16 >> alloc 15 17
-            regs $ alloc 20 18 >> alloc 19 19 >> alloc 18 20
-            regs $ alloc 23 21 >> alloc 22 22 >> alloc 21 23
-            regs $ alloc 26 24 >> alloc 25 25 >> alloc 24 26
-            regs $ alloc 29 27 >> alloc 28 28 >> alloc 27 29
-            regs $ alloc 32 30 >> alloc 31 31 >> alloc 30 32
+        regs $ alloc  2  0 >> alloc  1  1 >> alloc  0  2
+        regs $ alloc  5  3 >> alloc  4  4 >> alloc  3  5
+        regs $ alloc  8  6 >> alloc  7  7 >> alloc  6  8
+        regs $ alloc 11  9 >> alloc 10 10 >> alloc  9 11
+        regs $ alloc 14 12 >> alloc 13 13 >> alloc 12 14
+        regs $ alloc 17 15 >> alloc 16 16 >> alloc 15 17
+        regs $ alloc 20 18 >> alloc 19 19 >> alloc 18 20
+        regs $ alloc 23 21 >> alloc 22 22 >> alloc 21 23
+        regs $ alloc 26 24 >> alloc 25 25 >> alloc 24 26
+        regs $ alloc 29 27 >> alloc 28 28 >> alloc 27 29
+        regs $ alloc 32 30 >> alloc 31 31 >> alloc 30 29
+        regs $ alloc  2  0 >> alloc  1  1 >> alloc  0  2
+        regs $ alloc  5  3 >> alloc  4  4 >> alloc  3  5
+        regs $ alloc  8  6 >> alloc  7  7 >> alloc  6  8
+        regs $ alloc 11  9 >> alloc 10 10 >> alloc  9 11
+        regs $ alloc 14 12 >> alloc 13 13 >> alloc 12 14
+        regs $ alloc 17 15 >> alloc 16 16 >> alloc 15 17
+        regs $ alloc 20 18 >> alloc 19 19 >> alloc 18 20
+        regs $ alloc 23 21 >> alloc 22 22 >> alloc 21 23
+        regs $ alloc 26 24 >> alloc 25 25 >> alloc 24 26
+        regs $ alloc 29 27 >> alloc 28 28 >> alloc 27 29
+        regs $ alloc 32 30 >> alloc 31 31 >> alloc 30 29
